ironfleet/ravana/Service.i.dfy
@@ -1,0 +1,18 @@
+include "Types.i.dfy"
+
+module Service_i {
+  predicate Service_Init(s: ServiceState, switches: set<EndPoint>) {
+    s.outstandingCommands == {} &&
+    s.outstandingEvents == {} &&
+    keys_match(s.switchStates, switches)
+  }
+
+  predicate Service_Next(s: ServiceState, s': ServiceState) {
+    Service_NextNewEvent(s, s') ||
+    Service_NextApplyEvent(s, s') ||
+    Service_NextApplyCommand(s, s')
+  }
+
+  predicate Service_NextNewEvent(s: ServiceState, s': ServiceState) {
+  }
+}
